new: More changes

A3.dfy
@@ -1,19 +1,218 @@
+ghost function reverse_sequence<T>(s: seq<T>): seq<T> {
+    if |s| == 0 then [] else reverse_sequence(s[1..]) + [s[0]]
+}
+
 class Stack<T(0)> {
 
+    ghost var Elements: seq<T>
+    ghost const max: nat
+    ghost var Repr: set<object>
+
+    var size: nat
+    var stack: array<T>
+
+    ghost predicate Valid()
+        reads this, Repr
+        ensures Valid() ==> this in Repr && |Elements| <= max
+    {
+        // Preventing aliasing
+        this in Repr && stack in Repr &&
+        // Abstraction relation
+        |Elements| <= max &&
+        |Elements| == size &&
+        max == stack.Length &&
+        reverse_sequence(Elements) == stack[..size]
+    }
+
     constructor (max: nat)
+        ensures Valid() && fresh(Repr)
+        ensures Elements == [] && this.max == max
+    {
+        this.max := max;
+        Elements := [];
+        stack := new T[max];
+        size := 0;
+        Repr := {this, stack};
+    }
        
     predicate IsEmpty() 
+        requires Valid()
+        reads Repr
+        ensures Valid()
+        ensures IsEmpty() <==> |Elements| == 0
+        ensures !IsEmpty() <==> |Elements| != 0
+    {
+        size == 0
+    }
 
     method Push(v: T)
+        requires Valid() && |Elements| < max
+        modifies Repr
+        ensures Valid() && fresh(Repr - old(Repr))
+        ensures Elements == [v] + old(Elements)
+    {
+        stack[size] := v;
+        size := size + 1;
+        Elements := [v] + Elements;
+    }
 
     method Pop() returns (v: T)
+        requires Valid() && !IsEmpty()
+        modifies Repr
+        ensures Valid() && fresh(Repr - old(Repr))
+        ensures Elements == old(Elements[1..])
+        ensures v == old(Elements[0])
+    {
+        size := size - 1;
+        v := stack[size];
+        Elements := Elements[1..];
+    }
 }
 
 class Queue<T(0)> {
 
+    // abstract state
+    ghost var Elements: seq<T>
+    ghost const max: nat
+    ghost var Repr: set<object>
+
+    // concrete state
+    var stack1: Stack<T>
+    var stack2: Stack<T>
+
+    ghost predicate Valid()
+        reads this, Repr
+        ensures Valid() ==> this in Repr && |Elements| <= max
+    {
+        // Aliasing
+        this in Repr &&
+        (
+            stack1 in Repr &&
+            stack1.Repr <= Repr &&
+            this !in stack1.Repr
+        ) &&
+        (
+            stack2 in Repr &&
+            stack2.Repr <= Repr &&
+            this !in stack2.Repr
+        ) &&
+        stack1.Valid() && stack2.Valid() &&
+        stack1.Repr !! stack2.Repr &&
+        // Abstract relation
+        |Elements| <= max &&
+        Elements == stack1.Elements + reverse_sequence(stack2.Elements) &&
+        |Elements| == |stack1.Elements| + |stack2.Elements| &&
+        max == stack1.max &&
+        max == stack2.max
+    }
+
+
     constructor (max: nat)
+        ensures Valid() && fresh(Repr)
+        ensures Elements == [] && this.max == max
+    {
+        Elements := [];
+        this.max := max;
+        stack1 := new Stack<T>(max);
+        stack2 := new Stack<T>(max);
+        new;
+        Repr := {this, stack1, stack2} + stack1.Repr + stack2.Repr;
+    }
 
     method Add(v: T)
+        requires Valid() && |Elements| < max
+        modifies Repr
+        ensures Valid() && fresh(Repr - old(Repr))
+        ensures Elements == [v] + old(Elements)
+    {
+        Elements := [v] + Elements;
+        stack1.Push(v);
+        Repr := Repr + stack1.Repr;
+    }
     
     method Remove() returns (v:T)
+        requires Valid() && |Elements| > 0
+        modifies Repr
+        ensures Valid() && fresh(Repr - old(Repr))
+        ensures Elements == old(Elements[..|Elements|-1])
+        ensures v == old(Elements[|Elements|- 1])
+    // {
+    //     if stack2.IsEmpty() {
+    //         var temp: T;
+    //         assert stack1.Repr !! stack2.Repr;
+    //         while !stack1.IsEmpty()
+    //             decreases |stack1.Elements|
+    //             invariant stack1.Valid() && stack2.Valid() // This fixes the !stack1.IsEmpty() not meeting preconditions in loop gaurd
+    //             // Why does this happen?? Queue.Valid() includes stack1.Valid() and stack2.Valid() and the IsEmpty() requires and ensures Valid() for stack
+
+    //             invariant Elements == old(Elements) // Adding this resolves modifies clause error with v := stack2.Pop();
+    //             invariant |Elements| == |stack1.Elements| + |stack2.Elements| // Adding this resolves modifies clause error with v := stack2.Pop();
+    //             invariant Elements == stack1.Elements + reverse_sequence(stack2.Elements) // Adding this resolves modifies clause error with v := stack2.Pop();
+    //             // invariant stack1.Valid() && stack2.Valid() // Having these in there might violate modifies clause with v := stack2.Pop()???
+    //         {
+    //             // assert stack1.Repr !! stack2.Repr; // This is not holding for some reason
+    //             temp := stack1.Pop(); // With code currently, these are not holding - violate context's modifies clause
+    //             Repr := Repr + stack1.Repr;
+    //             stack2.Push(temp); // With code currently, these are not holding - violate context's modifies clause
+    //             Repr := Repr + stack2.Repr;
+    //         }
+    //     }
+    //     v := stack2.Pop();
+
+    //     Elements := Elements[..|Elements| - 1];
+    //     Repr := Repr + stack2.Repr + stack1.Repr;
+    // }
+}
+
+// method Main() {
+//     var check := new Queue<int>(5);
+
+//     assert |check.Elements| == 0;
+
+//     check.Add(5);
+//     check.Add(10);
+//     check.Add(10);
+//     check.Add(10);
+//     check.Add(10);
+
+//     var r1 := check.Remove();
+//     assert r1 == 5;
+
+//     check.Add(10);
+
+//     var r2 := check.Remove();
+//     assert r2 == 10;
+
+// }
+
+method Main() {
+    var check: seq<int>;
+
+    check := [1,2];
+
+    assert check == [1,2];
+
+    assert check == [1,2];
+    var check1 := reverse_sequence(check);
+    assert check1 == [2,1];
+
+    var a := new Stack<int>(5);
+    assert a.IsEmpty() == true;
+    a.Push(5);
+    assert a.IsEmpty() == false;
+    a.Push(10);
+    assert a.IsEmpty() == false;
+    a.Push(15);
+
+    var v1 := a.Pop();
+    assert v1 == 15;
+    var v2 := a.Pop();
+    assert v2 == 10;
+    var v3 := a.Pop();
+    assert v3 == 5;
+
+    a.Push(6);
+    var v4 := a.Pop();
+    assert a.IsEmpty() == true;
+    assert v4 == 6;
 }
